Better formalization for syntactic reduction.

SyntacticReduction.v
@@ -1,8 +1,9 @@
-Require Import Logic.LogicBase.
 Require Export Coq.Relations.Relation_Definitions.
 Require Export Coq.Relations.Relation_Operators.
 Require Export Coq.Relations.Relation_Definitions.
 Require Export Coq.Classes.RelationClasses.
+Require Import Logic.LogicBase.
+Require Import Logic.lib.Coqlib.
 
 Inductive propag_reduce {L: Language} (atomic_reduce: expr -> expr -> Prop): expr -> expr -> Prop :=
   propag_reduce_spec: forall x y p, atomic_reduce x y ->
@@ -12,67 +13,147 @@ Class SyntacticReduction (L: Language) : Type := {
   atomic_reduce: expr -> expr -> Prop;
   single_step_reduce := propag_reduce atomic_reduce;
   reduce := clos_refl_trans _ single_step_reduce
-(*
-  normal_form: expr -> Prop;
-  normal_form_spec1: forall x, normal_form x <-> ~ exists y, single_step_reduce x y;
-  reduce_function: expr -> expr;
-  reduce_function_sound: forall x, reduce x (reduce_function x);
-  reduce_function_normal: forall x, normal_form (reduce_function x);
-  atomic_reduce_preserve_reduce_function:
-    forall x y, atomic_reduce x y -> reduce_function x = reduce_function y;
-  single_propagation_preserve_reduce_function:
-    forall x y sp, reduce_function x = reduce_function y ->
-      reduce_function (single_propagation_denote sp x) = reduce_function (single_propagation_denote sp y)
-*)
 }.
 
-(*
-Lemma single_step_reduce_preserve_reduce_function {L: Language} {SD: SyntacticReduction L}:
-  forall x y, single_step_reduce x y -> reduce_function x = reduce_function y.
+Class NormalSyntacticReduction (L: Language) (R: SyntacticReduction L) : Type := {
+  normal_form: expr -> Prop;
+  reduce_to_norm: forall x, exists y, reduce x y /\ normal_form y
+}.
+
+Definition context_reduce {L: Language} {R: SyntacticReduction L} (Phi Psi: context): Prop :=
+  (forall x, Phi x -> exists y, reduce x y /\ Psi y) /\
+  (forall y, Psi y -> exists x, reduce x y /\ Phi x).
+
+Local Open Scope logic_base.
+
+Definition reduction_consistent_semantics {L: Language} (R: SyntacticReduction L) (SM: Semantics L): Prop :=
+  forall x y m, reduce x y -> (m |= x <-> m |= y).
+
+Definition reduction_consistent_prooftheory {L: Language} (R: SyntacticReduction L) (Gamma: ProofTheory L): Prop :=
+  (forall x y, reduce x y -> (|-- x <-> |-- y)) /\
+  (forall Phi Psi x y, context_reduce Phi Psi -> reduce x y -> (Phi |-- x <-> Psi |-- y)).
+
+Definition reduction_consistent_axiomization {L: Language} (R: SyntacticReduction L) (Gamma: AxiomaticProofTheory.AxiomaticProofTheory L): Prop :=
+  forall x y, reduce x y -> (AxiomaticProofTheory.provable x <-> AxiomaticProofTheory.provable y).
+
+(* Properties *)
+
+Lemma propagation_propagation_denote {L: Language}: forall p1 p2 x,
+  propagation_denote p1 (propagation_denote p2 x) = propagation_denote (p1 ++ p2) x.
+Proof.
+  intros.
+  induction p1.
+  + reflexivity.
+  + simpl.
+    f_equal; auto.
+Qed.
+
+Lemma propag_reduce_propag_reduce {L: Language}: forall r x y,
+  propag_reduce (propag_reduce r) x y -> propag_reduce r x y.
 Proof.
   intros.
   destruct H.
-  induction p; simpl.
-  + apply atomic_reduce_preserve_reduce_function; auto.
-  + apply single_propagation_preserve_reduce_function; auto.
+  destruct H.
+  rewrite !propagation_propagation_denote.
+  constructor; auto.
 Qed.
 
-Lemma reduce_preserve_reduce_function {L: Language} {SD: SyntacticReduction L}:
-  forall x y, reduce x y -> reduce_function x = reduce_function y.
+Lemma propag_reduce_reduce {L: Language} {R: SyntacticReduction L}: forall x y,
+  propag_reduce reduce x y -> reduce x y.
+Proof.
+  intros.
+  destruct H.
+  induction H.
+  + apply rt_step.
+    unfold single_step_reduce in *.
+    destruct H.
+    rewrite !propagation_propagation_denote.
+    constructor; auto.
+  + apply rt_refl.
+  + eapply rt_trans; eauto.
+Qed.
+
+Lemma reduce_step {L: Language} {R: SyntacticReduction L}:
+  forall x y, single_step_reduce x y -> reduce x y.
+Proof. intros. apply rt_step; auto. Qed.
+
+Lemma reduce_refl {L: Language} {R: SyntacticReduction L}:
+  forall x, reduce x x.
+Proof. intros. apply rt_refl; auto. Qed.
+
+Lemma reduce_trans {L: Language} {R: SyntacticReduction L}:
+  forall x y z, reduce x y -> reduce y z -> reduce x z.
+Proof. intros. eapply rt_trans; eauto. Qed.
+
+Lemma imp_reduce {L: Language} {nL: NormalLanguage L} {R: SyntacticReduction L}:
+  forall x1 x2 y1 y2,
+    reduce x1 x2 ->
+    reduce y1 y2 ->
+    reduce (impp x1 y1) (impp x2 y2).
+Proof.
+  intros.
+  eapply reduce_trans.
+  + apply propag_reduce_reduce.
+    rewrite <- imp1_propag_denote.
+    apply (propag_reduce_spec _ _ _ (imp1_propag y1 :: nil) H).
+  + simpl; rewrite imp1_propag_denote.
+    apply propag_reduce_reduce.
+    rewrite <- !imp2_propag_denote.
+    apply (propag_reduce_spec _ _ _ (imp2_propag x2 :: nil) H0).
+Qed.
+
+Lemma multi_imp_reduce {L: Language} {nL: NormalLanguage L} {R: SyntacticReduction L}:
+  forall xs1 xs2 y1 y2,
+    Forall2 reduce xs1 xs2 ->
+    reduce y1 y2 ->
+    reduce (multi_imp xs1 y1) (multi_imp xs2 y2).
 Proof.
   intros.
   induction H.
-  + apply single_step_reduce_preserve_reduce_function; auto.
-  + reflexivity.
-  + etransitivity; eauto.
+  + auto.
+  + simpl.
+    apply imp_reduce; auto.
 Qed.
 
-Lemma normal_form_spec2 {L: Language} {SD: SyntacticReduction L}:
-  forall x, normal_form x <-> reduce_function x = x.
+Lemma reduction_consistent_prooftheory_from_axiomization {L: Language} {nL: NormalLanguage L} (R: SyntacticReduction L) (Gamma: AxiomaticProofTheory.AxiomaticProofTheory L):
+  reduction_consistent_axiomization R Gamma ->
+  reduction_consistent_prooftheory R (AxiomaticProofTheory.G Gamma).
 Proof.
   intros.
-  split; intros.
-  + pose proof reduce_function_sound x.
-    rewrite normal_form_spec1 in H.
-    remember (reduce_function x) as y; clear Heqy.
-    induction H0.
-    - exfalso.
-      apply H; exists y; auto.
-    - auto.
-    - specialize (IHclos_refl_trans1 H).
-      subst y.
-      specialize (IHclos_refl_trans2 H).
-      auto.
-  + rewrite <- H; apply reduce_function_normal.
+  hnf in H |- *.
+  split; auto.
+  intros; simpl; split; intros; hnf in H2 |- *.
+  + destruct H2 as [xs [? ?]].
+    destruct H0.
+    pose proof fin_subset_match Phi Psi H0 xs H2.
+    destruct H5 as [ys [? ?]].
+    exists ys; split; auto.
+    erewrite <- H; eauto.
+    apply multi_imp_reduce; auto.
+  + destruct H2 as [ys [? ?]].
+    destruct H0.
+    pose proof fin_subset_match Psi Phi H4 ys H2.
+    destruct H5 as [xs [? ?]].
+    exists xs; split; auto.
+    erewrite H; eauto.
+    apply multi_imp_reduce; auto.
+    apply Forall2_lr_rev; auto.
 Qed.
 
-Lemma reduce_unique {L: Language} {SD: SyntacticReduction L}:
-  forall x y, normal_form y -> reduce x y -> reduce_function x = y.
+Theorem weak_completeness_reduce {L: Language} {nL: NormalLanguage L} (R: SyntacticReduction L) {nR: NormalSyntacticReduction L R} (Gamma: ProofTheory L) (SM: Semantics L):
+  reduction_consistent_prooftheory R Gamma ->
+  reduction_consistent_semantics R SM ->
+  (forall x, normal_form x -> |== x -> |-- x) ->
+  weakly_complete Gamma SM.
 Proof.
-  intros.
-  apply reduce_preserve_reduce_function in H0.
-  apply normal_form_spec2 in H.
-  congruence.
+  intros; hnf; intros.
+  destruct (reduce_to_norm x) as [y [? ?]].
+  specialize (H1 y H4).
+  rewrite (proj1 H x y H3).
+  apply H1.
+  intro m; specialize (H2 m).
+  rewrite (H0 x y m H3) in H2.
+  auto.
 Qed.
-
-*)
+  
+  
