lib/Coqlib.v
@@ -1,0 +1,26 @@
+Require Import Coq.Sets.Ensembles.
+Require Import Coq.Lists.List.
+
+Lemma fin_subset_match {A B: Type} {P: A -> B -> Prop}: forall (X: Ensemble A) (Y: Ensemble B),
+  (forall x, X x -> exists y, P x y /\ Y y) ->
+  forall xs, Forall (fun x => X x) xs -> exists ys, Forall2 P xs ys /\ Forall (fun y => Y y) ys.
+Proof.
+  intros.
+  induction xs as [| x0 xs].
+  + exists nil; split; constructor.
+  + inversion H0; subst.
+    specialize (IHxs H4).
+    destruct IHxs as [ys [? ?]].
+    specialize (H x0 H3).
+    destruct H as [y0 [? ?]].
+    exists (y0 :: ys).
+    split; constructor; auto.
+Qed.
+
+Lemma Forall2_lr_rev {A B: Type} {P: A -> B -> Prop}: forall xs ys,
+  Forall2 (fun y x => P x y) ys xs ->
+  Forall2 P xs ys.
+Proof.
+  intros.
+  induction H; auto.
+Qed.
