Makefile
@@ -4,4 +4,7 @@ COQC = coqc
 	@echo COQC $*.v
 	@$(COQC) -q -R "." -as Logic $*.v
 
-all: Wf.vo base.vo IPC.vo trivial.vo Kripke.vo enumerate.vo LogicBase.vo PropositionalLogic/Syntax.vo PropositionalLogic/ClassicalPropositionalLogic.vo
+all: Wf.vo base.vo IPC.vo trivial.vo Kripke.vo enumerate.vo LogicBase.vo SyntacticReduction.v \
+     PropositionalLogic/Syntax.vo PropositionalLogic/ClassicalPropositionalLogic.vo \
+     PropositionalLogic/TrivialSemantics.vo PropositionalLogic/Sound_Classical_Trivial.vo \
+     PropositionalLogic/Complete_Classical_Trivial.vo lib/Coqlib.vo
